Command case for ifc typechecker

examples/relational/ifc_interpreter.fst
@@ -1,5 +1,5 @@
 (*--build-config
-    options:--admit_fsi FStar.Set --z3timeout 15;
+    options:--admit_fsi FStar.Set --z3timeout 15 --print_effect_args;
     other-files:set.fsi heap.fst st.fst all.fst st2.fst distinct.fst ifc_ts.fst
   --*)
 
@@ -63,4 +63,62 @@ let rec tc_aexp e =
     let l = if l1 <= l2 then l2 else l1 in
     let s1 = sub_exp l1 l p1 in 
     let s2 = sub_exp l2 l p2 in 
-    (| l, convert l (bin_op_exp l s1 s2) |)
+    (| l, convert_exp l (bin_op_exp l s1 s2) |)
+
+
+(* Typechecking commands: we typecheck in a given context *)
+val tc_com : l:label -> c:com -> Tot (option (ni_com l)) (decreases c)
+let rec tc_com l c = 
+  match c with 
+
+  | Skip -> Some (sub_com top l skip_com)
+
+  | Assign x e -> 
+    let lx = label_fun x in 
+    if l <= lx then
+      let (| l', ni_e |) = tc_aexp e in 
+      if l' <= lx then 
+        let ni_e' = sub_exp l' lx ni_e in 
+        let ni_as = convert_com lx (assign_com x ni_e') in 
+        Some (sub_com lx l ni_as)
+      else
+        None
+    else
+      None
+
+  | Seq c1 c2 ->
+    let r1 = tc_com l c1 in   
+    let r2 = tc_com l c2 in 
+    if is_None r1 || is_None r2 then
+      None
+    else
+      Some (convert_com l (seq_com l (Some.v r1) (Some.v r2)))
+
+  | If e ct cf -> 
+    let (| l1, r1 |) = tc_aexp e in
+    if l1 <= l then 
+      None
+    else
+      let r2 = tc_com l1 ct in 
+      let r3 = tc_com l1 cf in 
+      if is_None r2 || is_None r3 then
+        None
+      else
+        let s = cond_com l1 r1 (Some.v r2) (Some.v r3) in 
+        Some (sub_com l1 l s)
+
+  | While e cb -> 
+    let (| l1, r1 |) = tc_aexp e in
+    if l1 <= l then 
+      None
+    else
+      let r2 = tc_com l1 cb in 
+      if is_None r2 then 
+        None
+      else
+        let s = loop_com l1 r1 (Some.v r2) in 
+        Some (sub_com l1 l s)
+
+
+
+
